Proofs/Rewrites.thy
@@ -13,22 +13,22 @@ fun replace_usages :: "ID \<Rightarrow> ID \<Rightarrow> IRGraph \<Rightarrow> I
 lemma replace_usages_effect:
   assumes "g' = replace_usages nid nid' g"
   shows "kind g' nid = RefNode nid'"
-  using assms replace_node_lookup replace_usages.simps IRNode.distinct(2069)
-  by (metis)
+  using assms replace_node_lookup replace_usages.simps
+  using IRNode.simps(2498) by presburger
 
 lemma replace_usages_changeonly:
   assumes "nid \<in> ids g"
   assumes "g' = replace_usages nid nid' g"
   shows "changeonly {nid} g g'"
   using assms unfolding replace_usages.simps
-  by (metis DiffI changeonly.elims(3) ids_some replace_node_unchanged)
+  by (metis add_changed add_node_def replace_node_def)
 
 lemma replace_usages_unchanged:
   assumes "nid \<in> ids g"
   assumes "g' = replace_usages nid nid' g"
   shows "unchanged (ids g - {nid}) g g'"
   using assms unfolding replace_usages.simps
-  by (smt (verit, del_insts) DiffE ids_some replace_node_unchanged unchanged.simps)
+  using assms(2) disjoint_change replace_usages_changeonly by presburger
 
 
 
@@ -61,16 +61,19 @@ lemma constantConditionTrue:
   shows "g', p \<turnstile> (ifcond, m, h) \<rightarrow> (t, m, h)"
 proof -
   have if': "kind g' ifcond = IfNode (nextNid g) t f"
-    by (metis IRNode.simps(989) assms(1) assms(2) constantCondition.simps(1) replace_node_lookup)
-  have "bool_to_val True = (IntVal 1 1)"
+    using IRNode.distinct(1041) assms(1) assms(2) constantCondition.simps(1) replace_node_lookup by presburger
+  have truedef: "bool_to_val True = (IntVal32 1)"
     by auto
   have "ifcond \<noteq> (nextNid g)"
-    by (metis IRNode.simps(989) assms(1) emptyE ids_some nextNidNotIn)
-  then have c': "kind g' (nextNid g) = ConstantNode (IntVal 1 1)"
-    using assms(2) replace_node_unchanged
-    by (metis DiffI IRNode.distinct(585) \<open>bool_to_val True = IntVal 1 1\<close> add_node_lookup assms(1) constantCondition.simps(1) emptyE insertE not_in_g)
+    by (metis IRNode.distinct(1041) assms(1) emptyE ids_some nextNidNotIn)
+  then have "kind g' (nextNid g) = ConstantNode (IRTreeEval.bool_to_val True)"
+    by (smt (z3) IRNode.distinct(641) add_changed add_node_def assms(1) assms(2) constantCondition.simps(1) not_in_g other_node_unchanged replace_node_def replace_node_lookup singletonD)
+  then have c': "kind g' (nextNid g) = ConstantNode (IntVal32 1)"
+    using truedef by simp
+  have "[g', m, p] \<turnstile> nextNid g \<mapsto> IntVal32 1"
+    by (metis ConstantExpr ConstantNode Value.distinct(1) \<open>kind g' (nextNid g) = ConstantNode (IRTreeEval.bool_to_val True)\<close> encodeeval_def truedef)
   from if' c' show ?thesis using IfNode
-    by (smt (z3) ConstantNode val_to_bool.simps(1))
+    by (metis (no_types, hide_lams) IRTreeEval.val_to_bool.simps(1) \<open>[g',m,p] \<turnstile> nextNid g \<mapsto> IntVal32 1\<close> encodeeval_def zero_neq_one)
 qed
 
 lemma constantConditionFalse:
@@ -79,16 +82,19 @@ lemma constantConditionFalse:
   shows "g', p \<turnstile> (ifcond, m, h) \<rightarrow> (f, m, h)"
 proof -
   have if': "kind g' ifcond = IfNode (nextNid g) t f"
-    by (metis IRNode.simps(989) assms(1) assms(2) constantCondition.simps(1) replace_node_lookup)
-  have "bool_to_val False = (IntVal 1 0)"
+    by (metis IRNode.simps(1090) assms(1) assms(2) constantCondition.simps(1) replace_node_lookup)
+  have falsedef: "bool_to_val False = (IntVal32 0)"
     by auto
   have "ifcond \<noteq> (nextNid g)"
-    by (metis IRNode.simps(989) assms(1) emptyE ids_some nextNidNotIn)
-  then have c': "kind g' (nextNid g) = ConstantNode (IntVal 1 0)"
-    using assms(2) replace_node_unchanged
-    by (metis DiffI IRNode.distinct(585) \<open>bool_to_val False = IntVal 1 0\<close> add_node_lookup assms(1) constantCondition.simps(1) emptyE insertE not_in_g)
+    by (metis IRNode.simps(1090) assms(1) equals0D ids_some nextNidNotIn)
+  then have "kind g' (nextNid g) = ConstantNode (IRTreeEval.bool_to_val False)"
+    by (smt (z3) IRNode.distinct(641) add_changed add_node_def assms(1) assms(2) constantCondition.simps(1) not_in_g other_node_unchanged replace_node_def replace_node_lookup singletonD)
+  then have c': "kind g' (nextNid g) = ConstantNode (IntVal32 0)"
+    using falsedef by simp
+  have "[g', m, p] \<turnstile> nextNid g \<mapsto> IntVal32 0"
+    by (metis ConstantExpr ConstantNode Value.distinct(1) \<open>kind g' (nextNid g) = ConstantNode (IRTreeEval.bool_to_val False)\<close> encodeeval_def falsedef)
   from if' c' show ?thesis using IfNode
-    by (smt (z3) ConstantNode val_to_bool.simps(1))
+    by (metis (no_types, hide_lams) IRTreeEval.val_to_bool.simps(1) \<open>[g',m,p] \<turnstile> nextNid g \<mapsto> IntVal32 0\<close> encodeeval_def)
 qed
 
 lemma diff_forall:
@@ -101,7 +107,7 @@ lemma replace_node_changeonly:
   shows "changeonly {nid} g g'"
   using assms replace_node_unchanged
   unfolding changeonly.simps using diff_forall
-  by (metis Rep_IRGraph_inverse add_changed add_node.rep_eq ids_some other_node_unchanged replace_node.rep_eq)
+  by (metis add_changed add_node_def changeonly.simps replace_node_def)
 
 lemma add_node_changeonly:
   assumes "g' = add_node nid node g"
@@ -137,7 +143,7 @@ proof (cases "is_IfNode (kind g nid)")
   then show ?thesis using assms
     using replace_node_changeonly add_node_changeonly unfolding changeonly.simps
     using True constantCondition.simps(1) is_IfNode_def
-    by (metis (full_types) DiffD2 Diff_insert_absorb)
+    by (metis (no_types, lifting) insert_iff)
 next
   case False
   have "g = g'"
@@ -161,14 +167,14 @@ qed
 
 lemma constantConditionValid:
   assumes "kind g ifcond = IfNode cond t f"
-  assumes "[g, m, p] \<turnstile> kind g cond \<mapsto> v"
+  assumes "[g, m, p] \<turnstile> cond \<mapsto> v"
   assumes "const = val_to_bool v"
   assumes "g' = constantCondition const ifcond (kind g ifcond) g"
   shows "\<exists>nid' .(g m p h \<turnstile> ifcond \<leadsto> nid') \<longleftrightarrow> (g' m p h \<turnstile> ifcond \<leadsto> nid')"
 proof (cases "const")
   case True
   have ifstep: "g, p \<turnstile> (ifcond, m, h) \<rightarrow> (t, m, h)"
-    by (meson IfNode True assms(1) assms(2) assms(3))
+    by (meson IfNode True assms(1) assms(2) assms(3) encodeeval_def)
   have ifstep': "g', p \<turnstile> (ifcond, m, h) \<rightarrow> (t, m, h)"
     using constantConditionTrue
     using True assms(1) assms(4) by presburger
@@ -177,7 +183,7 @@ proof (cases "const")
 next
   case False
   have ifstep: "g, p \<turnstile> (ifcond, m, h) \<rightarrow> (f, m, h)"
-    by (meson IfNode False assms(1) assms(2) assms(3))
+    by (meson IfNode False assms(1) assms(2) assms(3) encodeeval_def)
   have ifstep': "g', p \<turnstile> (ifcond, m, h) \<rightarrow> (f, m, h)"
     using constantConditionFalse
     using False assms(1) assms(4) by presburger
